\documentclass{article}
\usepackage{amsmath}
\usepackage{amssymb}
\usepackage{amstext}
\usepackage{ctex}
\begin{document}
\title{第四次作业}
\author{葛旭}
\maketitle
1.(1)$3a_1+a_2=a_3$\\
so $a_1,a_2,a_3$ is linearly dependent.\\
(2)suppose $k_1p_1(x)+k_2p_2(x)+k_3p_3(x)=0$,\\
so $k_1+5k_2+k_3=0 $\\
$-k_1+3k_2+3k_3=0$\\
$-2k_2+-2k_3=0$\\
figure out that $k_1=0,k_2=0,k_3=0$\\
so $p_1(x),p_2(x),p_3(x)$ is linearly independent\\
2.\[\begin{gathered}
  L({x_1} + {x_2}, \cdot  \cdot  \cdot ,{x_n} + {x_1}) = {k_1}({x_1} + {x_2}) +  \cdot  \cdot  \cdot  + {k_n}({x_n} + {x_1}) \hfill \\
   = ({k_1} + {k_n}){x_1} + ({k_1} + {k_2}){x_2} +  \cdot  \cdot  \cdot  + ({k_{n - 1}} + {k_n}){x_n} \hfill \\
  {x_1},{x_2}, \cdot  \cdot  \cdot ,{x_n}{\text{ is linearly independent,and n is an odd number,so }} \hfill \\
  \left\{ \begin{gathered}
  {k_1} + {k_n} = 0 \hfill \\
  {k_1} + {k_2} = 0 \hfill \\
   \cdot  \cdot  \cdot  \cdot  \cdot  \cdot  \cdot  \cdot  \cdot  \hfill \\
  {k_{n - 1}} + {k_n} = 0 \hfill \\
\end{gathered}  \right. \Rightarrow \left\{ \begin{gathered}
  {k_1} = 0 \hfill \\
  {k_2} = 0 \hfill \\
   \cdot  \cdot  \cdot  \cdot  \cdot  \cdot  \hfill \\
  {k_n} = 0 \hfill \\
\end{gathered}  \right. \hfill \\
  {\text{so }}{x_1} + {x_2}, \cdot  \cdot  \cdot  \cdot  \cdot  \cdot ,{x_n} + {x_1}{\text{ is linearly independent,too}}{\text{.}} \hfill \\
\end{gathered} \]
\end{document}